src/ecUnify.mli
@@ -51,7 +51,7 @@ type sbody = ((EcIdent.t * ty) list * expr) Lazy.t
 
 val select_op :
      ?hidden:bool
-  -> ?filter:(path -> operator -> bool)
+  -> ?filter:(EcPath.path -> operator -> bool)
   -> tvi
   -> EcEnv.env
   -> qsymbol
